Metrology/ProbLang/Test/DetStep.lean
@@ -6,11 +6,11 @@ namespace ProbLang
 open Lean Meta Elab
 
 /-! ## ToExpr instances for reflection -/
-deriving instance ToExpr for Binder
 deriving instance ToExpr for BaseLit
 deriving instance ToExpr for UnOp
 deriving instance ToExpr for BinOp
 deriving instance ToExpr for Ty
+deriving instance ToExpr for Binder
 deriving instance ToExpr for Annot
 deriving instance ToExpr for Exp
 deriving instance ToExpr for IsVal
